Exchange and fold

.CoqMakefile.d
@@ -7,9 +7,9 @@ lib/basics.vos lib/basics.vok lib/basics.required_vos: lib/basics.v acomputing/s
 lib/nvalues.vo lib/nvalues.glob lib/nvalues.v.beautified lib/nvalues.required_vo: lib/nvalues.v acomputing/syntax.vo
 lib/nvalues.vio: lib/nvalues.v acomputing/syntax.vio
 lib/nvalues.vos lib/nvalues.vok lib/nvalues.required_vos: lib/nvalues.v acomputing/syntax.vos
-lib/value_tree.vo lib/value_tree.glob lib/value_tree.v.beautified lib/value_tree.required_vo: lib/value_tree.v acomputing/syntax.vo
-lib/value_tree.vio: lib/value_tree.v acomputing/syntax.vio
-lib/value_tree.vos lib/value_tree.vok lib/value_tree.required_vos: lib/value_tree.v acomputing/syntax.vos
+lib/value_tree.vo lib/value_tree.glob lib/value_tree.v.beautified lib/value_tree.required_vo: lib/value_tree.v acomputing/syntax.vo lib/nvalues.vo
+lib/value_tree.vio: lib/value_tree.v acomputing/syntax.vio lib/nvalues.vio
+lib/value_tree.vos lib/value_tree.vok lib/value_tree.required_vos: lib/value_tree.v acomputing/syntax.vos lib/nvalues.vos
 lib/sensor_state.vo lib/sensor_state.glob lib/sensor_state.v.beautified lib/sensor_state.required_vo: lib/sensor_state.v acomputing/syntax.vo
 lib/sensor_state.vio: lib/sensor_state.v acomputing/syntax.vio
 lib/sensor_state.vos lib/sensor_state.vok lib/sensor_state.required_vos: lib/sensor_state.v acomputing/syntax.vos
@@ -19,9 +19,9 @@ acomputing/big_step_semantics.vos acomputing/big_step_semantics.vok acomputing/b
 test/basics_test.vo test/basics_test.glob test/basics_test.v.beautified test/basics_test.required_vo: test/basics_test.v lib/basics.vo lib/nvalues.vo acomputing/syntax.vo
 test/basics_test.vio: test/basics_test.v lib/basics.vio lib/nvalues.vio acomputing/syntax.vio
 test/basics_test.vos test/basics_test.vok test/basics_test.required_vos: test/basics_test.v lib/basics.vos lib/nvalues.vos acomputing/syntax.vos
-test/nvalues_test.vo test/nvalues_test.glob test/nvalues_test.v.beautified test/nvalues_test.required_vo: test/nvalues_test.v acomputing/syntax.vo lib/nvalues.vo
-test/nvalues_test.vio: test/nvalues_test.v acomputing/syntax.vio lib/nvalues.vio
-test/nvalues_test.vos test/nvalues_test.vok test/nvalues_test.required_vos: test/nvalues_test.v acomputing/syntax.vos lib/nvalues.vos
+test/nvalues_test.vo test/nvalues_test.glob test/nvalues_test.v.beautified test/nvalues_test.required_vo: test/nvalues_test.v acomputing/syntax.vo lib/nvalues.vo lib/value_tree.vo
+test/nvalues_test.vio: test/nvalues_test.v acomputing/syntax.vio lib/nvalues.vio lib/value_tree.vio
+test/nvalues_test.vos test/nvalues_test.vok test/nvalues_test.required_vos: test/nvalues_test.v acomputing/syntax.vos lib/nvalues.vos lib/value_tree.vos
 test/value_tree_test.vo test/value_tree_test.glob test/value_tree_test.v.beautified test/value_tree_test.required_vo: test/value_tree_test.v acomputing/syntax.vo lib/nvalues.vo lib/value_tree.vo
 test/value_tree_test.vio: test/value_tree_test.v acomputing/syntax.vio lib/nvalues.vio lib/value_tree.vio
 test/value_tree_test.vos test/value_tree_test.vok test/value_tree_test.required_vos: test/value_tree_test.v acomputing/syntax.vos lib/nvalues.vos lib/value_tree.vos
