test/nvalues_test.v
@@ -1,12 +1,19 @@
 Require Import PeanoNat.
 From AC Require Import syntax.
 From AC Require Import nvalues.
+From AC Require Import value_tree.
+Require Import String.
+Require Import List.
 
+Definition x : string := "x".
+Definition y : string := "y".
+Definition fun0: string := "fun0". 
+Definition fun1: string := "fun1".
 
-Compute (get 0 <{[0>>6][>5]}>).
-Compute (get 1 <{[0>>6][>5]}>).
-Compute (get 2 <{[0>>6][2>>7][>5]}>).
-Compute (getDefault <{[0>>6][2>>7][>5]}>).
+Compute (nvalues.get 0 <{[0>>6][>5]}>).
+Compute (nvalues.get 1 <{[0>>6][>5]}>).
+Compute (nvalues.get 2 <{[0>>6][2>>7][>5]}>).
+Compute (nvalues.getDefault <{[0>>6][2>>7][>5]}>).
 
 Lemma first: ordered (default 5).
 Proof.
@@ -33,3 +40,4 @@ Compute (extend (device  1 2(device  3 5(device  5 7(device  7 3(default  1)))))
 
 Compute (extend (device  2 2(device  4 5(device  6 7(device  7 3(default  2)))))  (device  1 2(device  3 5(device  5 7(device  7 3 (default  1)))))).
 
+Compute (folding 4 (rev (devices (vt_el 4 (empty nil) (vt_el 5 (empty nil) vt_end)))) <{[ > fun fun0[x:Nat] {fun fun0[y:Nat] {x*y} }]}>  <{[4 >> 2][5 >> 6][> 7]}> <{[>6]}> ).
