acomputing/syntax.v
@@ -1,20 +1,29 @@
+(** ** SYNTAX 
+    In this section we define the syntax of the aggregate computing calculus
+    The syntax, as for the semantics, is similar to the lambda calculus.
+*)
+
+
 Set Warnings "-notation-overridden,-parsing,-deprecated-hint-without-locality".
 Require Import Strings.String.
 Require Import PeanoNat.
 Require Import Bool.
 Require Import List.
 
+(** The identifier of a device is seen as natural number*)
 Definition ident := nat.
 
 Inductive ty : Type :=
   | Ty_Builtin : Type -> ty
   | Ty_Arrow : ty -> ty -> ty.
 
+(** SYNTAX of an EXPRESSION, including LITERALS and NVALUES*)
+(** An expression can be a 
+variable (rappresented by string), .... *)
 Inductive exp: Type :=
   | exp_var : string -> exp
   | exp_app : exp -> exp -> exp
   | exp_val : string -> exp -> exp -> exp
-  | exp_if : exp -> exp -> exp -> exp
   | exp_nvalue : nvalue -> exp
   | exp_literal : literal -> exp
 with literal :=
@@ -27,21 +36,20 @@ with literal :=
   | l_const : nat -> literal
   | l_succ : exp -> literal
   | l_pred : exp -> literal 
+  | l_abs : string -> string -> ty -> exp -> literal 
   | l_mult : exp -> exp -> literal
-  | l_abs : string -> string -> ty -> exp -> literal
   | l_nfold : exp -> exp -> exp -> literal
-  | l_nvalue_get: exp -> exp -> literal
-  | l_nvalue_getDefault: exp -> literal
+  | l_exchange : exp -> exp -> literal
 with nvalue :=
   | default: literal -> nvalue
   | device (n:ident) : literal -> nvalue -> nvalue.
 
 Declare Custom Entry acnotation.
 
-(*expresion*)
+(** In order to make an expresion more undestandable we define a notation for syntax, including
+nvalues*)
 Notation "<{ e }>" := e (e custom acnotation at level 99).
 
-(*lambda*)
 Notation "'fun' name [ x :  t ]  { y }" :=
   (l_abs name x t y) (in custom acnotation at level 90, 
                      name at level 99,
@@ -51,7 +59,6 @@ Notation "'fun' name [ x :  t ]  { y }" :=
                      name at level 99,
                      left associativity).
 
-(*application*)
 Notation "x y " := (exp_app x y) (in custom acnotation at level 1, left associativity).
 Notation "( x )" := x (in custom acnotation, x at level 99).
 Notation "x" := x (in custom acnotation at level 0, x constr at level 0).
@@ -64,7 +71,6 @@ Notation "'val' name = x ; y" := (exp_val name x y) (in custom acnotation at lev
 
 Notation "S -> T" := (Ty_Arrow S T) (in custom acnotation at level 50, right associativity).
 
-(*boolean*)
 Notation "'Bool'" := (Ty_Builtin bool) (in custom acnotation at level 0).
 Notation "'true'" := true (at level 1).
 Notation "'true'" := l_true (in custom acnotation at level 0).
@@ -79,24 +85,16 @@ Notation "'pred' x" := (l_pred x) (in custom acnotation at level 0,
                                      x custom acnotation at level 0).
 Notation "x * y" := (l_mult x y) (in custom acnotation at level 1,
                                       left associativity).
-Notation "'nv_get' pos nv" := (l_nvalue_get pos nv) (in custom acnotation at level 0,
-                                     nv custom acnotation at level 0,
-                                     pos custom acnotation at level 0).
-Notation "'nv_default' x" := (l_nvalue_getDefault x) (in custom acnotation at level 0,
-                                     x custom acnotation at level 0).
 
 Notation "'nfold' e0 e1 e2" := (l_nfold e0 e1 e2) (in custom acnotation at level 0,
                                      e0 custom acnotation at level 0,
                                      e1 custom acnotation at level 0,
                                      e2 custom acnotation at level 0).
 
-(*if condition*)
-Notation "'if' x 'then' y 'else' z" :=
-  (exp_if x y z) (in custom acnotation at level 89,
-                    x custom acnotation at level 99,
-                    y custom acnotation at level 99,
-                    z custom acnotation at level 99,
-                    left associativity).
+Notation "'exchange' e0 e1" := (l_exchange e0 e1) (in custom acnotation at level 0,
+                                     e0 custom acnotation at level 0,
+                                     e1 custom acnotation at level 0).
+
 
 (*nvalues*)
 Notation "[ > l ]" := (default l) (in custom acnotation at level 30).
@@ -106,10 +104,14 @@ Notation "[ x >> y ] m" := ( device x y m)(in custom acnotation at level 30,
                                             m custom acnotation at level 30).
 
 Notation "'FAIL'" := (l_fail) (in custom acnotation at level 0).
+
 Notation "'sensor' x" := (l_sensor x) (in custom acnotation at level 0, x custom acnotation at level 0).
+
 Notation "'self' x" := (l_self x) (in custom acnotation at level 0, x custom acnotation at level 0).
+
 Notation "'uid'" := (l_uid) (in custom acnotation at level 0).
 
+(** EXPRESS CONCEPT*)
 Coercion exp_var : string >-> exp.
 Coercion exp_literal: literal >-> exp.
 Coercion l_const: nat >-> literal.
