lib/nvalues.v
@@ -1,5 +1,6 @@
 Require Import PeanoNat.
 From AC Require Import syntax.
+Require Import List.
 
 (*get single device value*)
 Fixpoint get (pos:ident) (n:nvalue): literal :=
@@ -45,55 +46,10 @@ end.
 
 
 
-(*
-Compute (extend (device nat 1 2 (device nat 5 4 (device nat 7 6 (default nat 8))))  
-(device nat 0 1 (device nat 1 3 (device nat 3 5 (device nat 4 7 (device nat 5 9 (device nat 6 11 ( device nat 8 13 ((default nat 6)))))))))).
-
-
-Fixpoint defaultV {A} (n:nvalue A): A :=
-match n with
-| default _ x => x
-| device _ _ _ m => defaultV m
+Fixpoint folding (delta:ident) (devs:list nat) (w1:nvalue) (w2:nvalue) (w3:nvalue) : exp :=
+match devs with 
+| cons id l => if (delta =? id) then (folding id l w1 w2 w3) else exp_app (exp_app w1 (nvalues.get id w2)) (folding delta l w1 w2 w3)
+| nil => (get delta w3)
 end.
-(*Operation between two nvalues*)
-(*A is the type of nvalue, op is the point-wise operation*)
-(*nvalues need to be ordered, this is achieved by a properly insertion in the data type*)
-(*It's possible to define a pointwise operation on non order nvalues,
-but we must to assure that the nvalue don't contains duplicates*)
-Fixpoint pointWise {A} (op:A->A->A) (w0:nvalue A) {struct w0}: nvalue A -> nvalue A:=
-fix pointWise1 (w1:nvalue A) {struct w1}: nvalue A :=
-match w0,w1 with
-| default _ x , default _ y => default A (op x y)
-| default _ x , device _ a b m  =>  device A a b (pointWise1 m) 
-| device _ a b m , default _ x  => device A a b (pointWise op  m (default A x)) 
-| device _ a0 b0 m0 , device _ a1 b1 m1  => if (a0=?a1) then device A a0 (op b0 b1) (pointWise op m0 m1)
-                                            else (if (a0<?a1) then device A a0 (op b0 (defaultV m1)) (pointWise op m0 (device A a1 b1 m1))
-                                            else device A a1 (op (defaultV m0) b1) (pointWise1 m1 ))
-end.
-
-
-(*check*)
-Definition int_sum (x:nat) (y:nat) : nat :=  x + y.
-Compute(pointWise int_sum (device nat 1 2(device nat 3 5(device nat 5 7(device nat 7 3(default nat 1))))) (device nat 2 2(device nat 4 5(device nat 6 7(device nat 7 3(default nat 2)))))).
-
-
-
-
-Lemma first: ordered (default nat 5).
-Proof.
-apply ordered0.
-Qed.
-
-Lemma second: ordered(device nat 3 5(default nat 4)).
-Proof.
-apply ordered1.
-Qed.
-
-Search lt.
-Lemma third: ordered(device nat 2 5(device nat 3 5(default nat 4))).
-Proof.
-apply ordered2. apply Nat.lt_succ_diag_r. apply ordered1.
-Qed.
-*)
 
 
