lib/value_tree.v
@@ -2,10 +2,17 @@ From AC Require Import syntax.
 Require Import String. 
 Require Import PeanoNat. 
 Require Import List. 
+Require Import nvalues.
 
 Inductive value_tree: Type :=
 | empty : list value_tree -> value_tree
 | some : nvalue -> list value_tree  -> value_tree.
+
+Definition rho (v:value_tree) : nvalue :=
+match v with 
+| empty _ => default l_fail
+| some w _ => w
+end.
 
 Definition extract_l (v:value_tree) : list value_tree:= 
 match v with 
@@ -33,9 +40,43 @@ match v_env with
 | (vt_el id vt vt_next) => vt_el id (pi pos vt) (pi_env pos vt_next)
 end.  
 
+Fixpoint devices (env:value_tree_env) : list nat :=
+match env with 
+| vt_el id _  vl => cons id (devices vl)
+| vt_end => nil
+end.
+
+Definition name_f (e:exp): option string :=
+match e with
+| <{fun n[x:T] {m}}> => Some n
+| _ => None
+end.
+
+Fixpoint select_f (v_env:value_tree_env) (e:exp) : value_tree_env :=
+match v_env with
+| vt_el id vt v_env_next => match (name_f (nvalues.get id (rho vt) )),(name_f e) with
+                            | Some n0, Some n1 => if (String.eqb n0 n1) then 
+                                                  (vt_el id vt (select_f v_env_next e)) else
+                                                  select_f v_env_next e
+                            | _ , _ => select_f v_env_next e (*? OR FAIL*)
+                            end
+| vt_end => vt_end 
+end.
+
+Fixpoint get_messages (my_id:ident) (w_i:nvalue) (v_env:value_tree_env) : nvalue :=
+match v_env with
+| vt_el id vt v_env_next => device id (nvalues.get my_id (rho vt)) (get_messages my_id w_i v_env_next) 
+| v_end => default (nvalues.getDefault w_i) (*nvalue dentro nvalue ?*)
+end.
+(* Se dentro a un nvalue di un value_tree non è presente 
+il valore per il nostro dispositivo è sufficiente il default? *)
 
 
+Compute (get_messages 2 <{[>5]}> (vt_el 3 (some <{[2>>5][>6]}> nil) 
+(vt_el 4 (some <{[1>>2][2>>6][>7]}> nil) (vt_el 7 (some <{[1>>2][2>>6][>7]}> nil) vt_end ) )  )).
 
+Compute (get_messages 2 <{[>5]}> (vt_el 3 (some <{[2>>5][>6]}> nil) 
+(vt_el 4 (some <{[1>>2][2>>6][>7]}> nil) (vt_el 7 (empty nil) vt_end ) )  )).
 
 
 
