test/big_step_semantics_test.v
@@ -12,7 +12,7 @@ Definition y : string := "y".
 Definition z : string := "z".
 Definition n : string := "n".
 Definition fun0: string := "fun0". 
-Definition prod5: string := "prod5". 
+Definition fun1: string := "fun1". 
 
 Hint Unfold x : core.
 Hint Unfold y : core.
@@ -27,3 +27,158 @@ apply A_MULT.
 -simpl. apply E_NVAL. 
 split. apply ordered2. auto. apply ordered1. apply w_device. apply v_nat. apply w_device. apply v_nat. apply w_default. apply v_nat.
 Qed.
+
+Lemma fold00: <[ 4 | base | vt_el 2 (empty nil) (vt_el 3 (empty nil) (vt_end)) | <{ nfold [> fun fun0[x:Nat] {fun fun0[y:Nat] {x*y} }] [2>>4][3>>5][>6] [>7] }> ]> ==> <[ <{[>140]}> | empty nil ]>.
+Proof.
+eapply A_FOLD.
+-split. 
++ apply ordered0.
++ apply w_default. apply v_abs. simpl. split. right. left. reflexivity. left. reflexivity.
+-split. 
++apply ordered2. auto. apply ordered1.
++ apply w_device. apply v_nat. apply w_device. apply v_nat. apply w_default. apply v_nat.
+-split. 
++ apply ordered0.
++ apply w_default. apply v_nat.
+- apply v_nat.
+- simpl. apply E_APP with (w0:=<{[> fun fun0 [y : Nat] { [>5] * y}]}>) (w1:=<{[>28]}>).
++ split. apply ordered0. apply w_default. apply v_abs. simpl. auto.
++ split. apply ordered0. apply w_default. apply v_nat.
++ split. apply ordered0. apply w_default. apply v_nat.
++ simpl. auto. 
++ apply func.
+
++ apply E_APP with (w0:=<{[ > fun fun0 [x : Nat] {fun fun0 [y : Nat] {x * y}}]}>) (w1:=<{[>5]}>).
+split. apply ordered0. apply w_default. apply v_abs. simpl. split. right. left. reflexivity. left. reflexivity.
+split. apply ordered0. apply w_default. apply v_nat. 
+split. apply ordered0. apply w_default. apply v_abs. simpl. auto. 
+simpl. auto. apply func. 
+apply E_NVAL.
+split. apply ordered0. apply w_default. apply v_abs. simpl. split. right. left. reflexivity. left. reflexivity.
+apply E_LIT. apply v_nat. 
+apply A_FUN. split. apply ordered0. apply w_default. apply v_nat. split. apply ordered0. apply w_default. apply v_abs. simpl. auto.
+simpl. apply E_LIT.  apply v_abs. simpl. auto.
+
++ apply E_APP with (w0:=<{[ > fun fun0 [y : Nat] {[>4] * y}]}>) (w1:=<{[>7]}>).
+split. apply ordered0. apply w_default. apply v_abs. simpl. auto.
+split. apply ordered0. apply w_default. apply v_nat.
+split. apply ordered0. apply w_default. apply v_nat.
+simpl. auto. apply func. 
+apply E_APP with (w0:=<{[ > fun fun0 [x : Nat] {fun fun0 [y : Nat] {x * y}}]}>) (w1:=<{[>4]}>).
+split. apply ordered0. apply w_default. apply v_abs. simpl. split. right. left. reflexivity. left. reflexivity.
+split. apply ordered0. apply w_default. apply v_nat.
+split. apply ordered0. apply w_default. apply v_abs. simpl. auto.
+simpl. auto. apply func. apply E_NVAL. 
+split. apply ordered0. apply w_default. apply v_abs. simpl. split. right. left. reflexivity. left. reflexivity.
+apply E_LIT. apply v_nat. apply A_FUN. split. apply ordered0. apply w_default. apply v_nat.
+split. apply ordered0. apply w_default. apply v_abs. simpl. auto. simpl. 
+apply E_LIT. apply v_abs. simpl. auto. 
+apply E_LIT. apply v_nat.
+apply A_FUN. split. apply ordered0. apply w_default. apply v_nat.
+split. apply ordered0. apply w_default. apply v_nat.
+simpl. apply A_MULT. 
+split. apply ordered0. apply w_default. apply v_nat.
+split. apply ordered0. apply w_default. apply v_nat.
+split. apply ordered0. apply w_default. apply v_nat.
+simpl. apply E_NVAL. split. apply ordered0. apply w_default. apply v_nat.
+
++apply A_FUN. split. apply ordered0. apply w_default. apply v_nat.
+split. apply ordered0. apply w_default. apply v_nat.
+simpl. apply A_MULT.  
+split. apply ordered0. apply w_default. apply v_nat.
+split. apply ordered0. apply w_default. apply v_nat.
+split. apply ordered0. apply w_default. apply v_nat.
+simpl. apply E_NVAL. split. apply ordered0. apply w_default. apply v_nat.
+
+Qed.
+
+
+Lemma fold00_R: <[ 4 | base | vt_el 2 (empty nil) (vt_el 3 (empty nil) (vt_end)) | <{ nfold [> fun fun0[x:Nat] {fun fun0[y:Nat] {x*y} }] [2>>4][3>>5][>6] [>7] }> ]> ==> <[ <{[>140]}> | empty nil ]>.
+Proof. 
+(*C0 call*)
+eapply A_FOLD_R with (l0:=<{28}>).
+(*C0: Preconditions*) 
+auto. split. apply ordered0. apply w_default. apply v_abs. simpl. auto.
+split. apply ordered2. auto. apply ordered1. apply w_device. apply v_nat. apply w_device. apply v_nat. apply w_default. apply v_nat.
+split. apply ordered0. apply w_default. apply v_nat.
+apply v_nat.
+apply v_nat.
+(*C0: Exteternal application E_APP0*)
+simpl. apply E_APP with (w0:=<{[>fun fun0 [y : Nat] {[>4] * y}]}>) (w1:=<{[>7]}>).
+(*C0: E_APP0:  Preconditions*)
+split. apply ordered0. apply w_default. apply v_abs. simpl. auto.
+split. apply ordered0. apply w_default. apply v_nat.
+split. apply ordered0. apply w_default. apply v_nat.
+simpl. auto. apply func.
+(*C0: E_APP0: Internal application I_APP0 e1 ==> w1*)
+apply E_APP with (w0:=<{[> fun fun0[x:Nat] {fun fun0[y:Nat] {x*y} }]}>) (w1:=<{[>4]}>).
+(*C0: E_APP0: I_APP0 Preconditions*)
+split. apply ordered0. apply w_default. apply v_abs. simpl. auto.
+split. apply ordered0. apply w_default. apply v_nat.
+split. apply ordered0. apply w_default. apply v_abs. simpl. auto.
+simpl. auto. apply func. 
+(*C0: E_APP0: I_APP0 e0 ==> w0*)
+apply E_NVAL. split. apply ordered0. apply w_default. apply v_abs. simpl. auto.
+(*C0: E_APP0: I_APP0 e1 ==> w1*)
+apply E_LIT. apply v_nat.
+(*C0: E_APP0: I_APP0 function f w1 => w2*)
+apply A_FUN. 
+split. apply ordered0. apply w_default. apply v_nat.
+split. apply ordered0. apply w_default. apply v_abs. simpl. auto.
+simpl. apply E_LIT. apply v_abs. simpl. auto.
+(*C0: E_APP0: e1 ==> w1*)
+apply E_NVAL. split. apply ordered0. apply w_default. apply v_nat.
+(*C0: E_APP0: I_APP0 function f w1 ==> w2*)
+apply A_FUN. 
+split. apply ordered0. apply w_default. apply v_nat.
+split. apply ordered0. apply w_default. apply v_nat.
+simpl. 
+apply A_MULT. 
+split. apply ordered0. apply w_default. apply v_nat.
+split. apply ordered0. apply w_default. apply v_nat.
+split. apply ordered0. apply w_default. apply v_nat.
+simpl. apply E_NVAL. split. apply ordered0. apply w_default. apply v_nat.
+(*C0: Recursive call C1*)
+eapply A_FOLD_B.
+(*C0:C1: Preconditions*)
+auto.
+split. apply ordered0. apply w_default. apply v_abs. simpl. auto.
+split. apply ordered2. auto. apply ordered1. apply w_device. apply v_nat. apply w_device. apply v_nat.
+  apply w_default. apply v_nat.
+split. apply ordered0. apply w_default. apply v_nat. 
+apply v_nat.
+(*C0: C1: External application E_APP01*)
+simpl. eapply E_APP with (w0:=<{[>fun fun0 [y : Nat] {[>5] * y}]}>) (w1:=<{[>28]}>).
+(*C0: C1: E_APP01: Preconditions*)
+split. apply ordered0. apply w_default. apply v_abs. simpl. auto.
+split. apply ordered0. apply w_default. apply v_nat.
+split. apply ordered0. apply w_default. apply v_nat.
+simpl. auto. apply func.
+(*C0: C1: E_APP01: Internal application I_APP01 e0==>w0*)
+eapply E_APP with (w0:=<{[>fun fun0[x:Nat] {fun fun0[y:Nat] {x*y} }]}>) (w1:=<{[>5]}>).
+(*C0: C1: E_APP01: I_APP01: Preconditions*)
+split. apply ordered0. apply w_default. apply v_abs. simpl. auto.
+split. apply ordered0. apply w_default. apply v_nat.
+split. apply ordered0. apply w_default. apply v_abs. simpl. auto.
+simpl. auto. apply func.
+(*C0: C1: E_APP01: I_APP01: e0 ==> w0*)
+apply E_NVAL. split. apply ordered0. apply w_default. apply v_abs. simpl. auto.
+(*C0: C1: E_APP01: I_APP01: e1 ==> w1*)
+apply E_LIT. apply v_nat.
+(*C0: C1: E_APP01: I_APP01: function f w1 ==> w2*)
+apply A_FUN. 
+split. apply ordered0. apply w_default. apply v_nat.
+split. apply ordered0. apply w_default. apply v_abs. simpl. auto.
+simpl. apply E_LIT. apply v_abs. simpl. auto.
+(*C0: C1: E_APP01: e1 ==> w1 *)
+apply E_NVAL. split. apply ordered0. apply w_default. apply v_nat.
+(*C0: C1: E_APP01: function f f w1 ==> w2 *)
+apply A_FUN. split. apply ordered0. apply w_default. apply v_nat.
+split. apply ordered0. apply w_default. apply v_nat.
+simpl. 
+apply A_MULT. 
+split. apply ordered0. apply w_default. apply v_nat.
+split. apply ordered0. apply w_default. apply v_nat.
+split. apply ordered0. apply w_default. apply v_nat.
+simpl. apply E_NVAL.  split. apply ordered0. apply w_default. apply v_nat.
+
