test/value_tree_test.v
@@ -50,3 +50,30 @@ Compute (pi_env 2 vt_env_0).
 
 Compute (pi_env 3 vt_env_0).
 
+(*Test name_f*)
+Definition pop:string:="pop".
+Definition top:string:="top".
+Definition x:string:="x".
+Compute (name_f <{fun pop[x:Nat] {5} }>).
+Compute (name_f <{x}>).
+
+(*Test select_f*)
+
+Compute (select_f  (vt_el 5 (some <{[>fun pop[x:Nat] {5}]}> nil ) 
+(vt_el 6 (some <{[>fun pop[x:Nat] {5}]}> nil ) vt_end ) )  <{fun pop[x:Nat] {5} }>).
+
+Compute (select_f  (vt_el 5 (some <{[>fun pop[x:Nat] {5}]}> nil ) 
+(vt_el 6 (some <{[>fun top[x:Nat] {5}]}> nil ) vt_end ) )  <{fun pop[x:Nat] {5} }>).
+
+Compute (select_f  (vt_el 5 (some <{[>fun pop[x:Nat] {5}]}> nil ) 
+(vt_el 6 (some <{[>6]}> nil ) vt_end ) )  <{fun pop[x:Nat] {5} }>).
+
+(*Test get_messages*)
+
+Compute (get_messages 2 <{[>5]}> (vt_el 3 (some <{[2>>5][>6]}> nil) 
+(vt_el 4 (some <{[1>>2][2>>6][>7]}> nil) (vt_el 7 (some <{[1>>2][2>>6][>7]}> nil) vt_end ) )  )).
+
+Compute (get_messages 2 <{[>5]}> (vt_el 3 (some <{[2>>5][>6]}> nil) 
+(vt_el 4 (some <{[1>>2][2>>6][>7]}> nil) (vt_el 7 (empty nil) vt_end ) )  )).
+
+
